coq/Rel.v
@@ -1,0 +1,129 @@
+(*===========================================================================
+    Binary relations
+  ===========================================================================*)
+Import Coq.Init.Notations.
+
+Require Export Coq.Classes.Morphisms.
+Require Export Relations.
+
+Section RelDefs.
+  Variable A B:Type.
+  Variable R R':relation A.
+  Variable S:relation B.
+
+  Definition difunctional := forall x x' y y', R x y -> R x' y' -> R x y' -> R x' y.
+
+  (* Relation constructions *)
+  Definition RelId    := (fun x y => x=y) : relation A.
+  Definition RelArrow := (fun f g : A->B =>
+    forall x y, R x y -> S (f x) (g y)) : relation (A->B).
+  Definition RelProd  := (fun x y : A*B => 
+     R (fst x) (fst y) /\ S (snd x) (snd y)) : relation (A*B).
+  Definition RelSum :=  (fun x y : A+B =>
+    match x with 
+    | inl x1 => match y with inl y1 => R x1 y1 | inr y2 => False end
+    | inr x2 => match y with inl y1 => False | inr y2 => S x2 y2 end
+    end) : relation (A+B).
+
+  (* Composition and inversion *)
+  Definition RelComp := (fun x y => exists z, R x z /\ R' z y) : relation A.
+
+  (* Relation equality *)
+  Definition RelEq := forall x y, R x y <-> R' x y.
+
+End RelDefs.
+
+Implicit Arguments RelId [].
+Implicit Arguments difunctional. 
+Implicit Arguments RelComp [A]. 
+Implicit Arguments RelArrow.
+Implicit Arguments RelProd. 
+Implicit Arguments RelSum. 
+Implicit Arguments RelEq.
+
+Bind Scope rel_scope with relation.
+Open Scope rel_scope.
+
+Notation "R * S" := (RelProd R S) : rel_scope.
+Notation "R + S" := (RelSum R S) : rel_scope.
+Notation "R 'o' S" := (RelComp R S) (at level 60, right associativity) : rel_scope.
+
+(*
+Ltac UnfoldRel := unfold RelProd, RelSum, Relation_Definitions.respectful, RelId, RelComp, RelInv, symmetric, transitive, reflexive, PER, difunctional.
+Ltac UnfoldRelAll := unfold RelProd, RelSum, RelArrow, RelId, RelComp, RelInv, symmetric, transitive, reflexive, PER, difunctional in *.
+*)
+
+Section RelLemmas.
+  Variable A B : Type.
+  Variable R : relation A.
+  Variable S : relation B.
+
+(*
+  Lemma id_PER : PER (RelId A). 
+  Proof. split; congruence. Qed.
+*)
+
+  Open Scope signature_scope.
+  Lemma arrow_symmetric: symmetric _ R -> symmetric _ S -> symmetric _ (R ==> S).
+  Proof. firstorder. Qed.
+
+  Lemma arrow_transitive : symmetric _ R -> transitive _ R -> transitive _ S -> transitive _ (R ==> S).
+  Proof.
+    intros Rsym Rtran Stran f g h H1 H2.
+    intros x z H3.
+    assert (R z x) by (apply Rsym; assumption).
+    assert (R x x) by firstorder.
+    firstorder.
+  Qed.
+
+(*
+  Lemma arrow_PER : PER R -> PER S -> PER (R ==> S).
+  Proof.
+    UnfoldRel.
+    split.
+    apply arrow_transitive; intuition.
+    apply arrow_symmetric; intuition.
+  Qed.
+
+  Lemma prod_PER : PER R -> PER S -> PER (R * S).
+  Proof. firstorder. Qed.
+*)
+
+  Lemma prod_difunctional : difunctional R -> difunctional S -> difunctional (R * S).
+  Proof.
+    intros RH SH.
+    unfold difunctional in *. unfold RelProd.
+    intros p p' q q' pq p'q' pq'.  
+    destruct pq as [pq1 pq2].
+    destruct p'q' as [p'q'1 p'q'2].
+    destruct pq' as [pq'1 pq'2].
+    eauto.
+  Qed.
+
+  Lemma arrow_difunctional : difunctional S -> difunctional (R ==> S).
+  Proof.
+    intros SH.
+    unfold difunctional, respectful in *.
+    intros x x' y y' xy x'y' xy'.
+    intros a b ab.
+    eauto.
+  Qed.
+
+  Lemma sum_difunctional : difunctional R -> difunctional S -> difunctional (R + S).
+  Proof.
+    intros RH SH.
+    unfold difunctional, RelSum in *.
+    intros s s' t t' st s't' st'. 
+    destruct s as [sl | sr].
+    destruct s' as [s'l | s'r]. destruct t as [tl | tr]. destruct t' as [t'l | t'r].
+    apply (RH sl s'l tl t'l); intuition. intuition. intuition. intuition.
+    destruct t' as [t'l | t'r]. intuition. intuition.
+    destruct t as [tl | tr].
+    destruct t' as [t'l | t'r]. intuition. intuition. intuition.
+    destruct t' as [t'l | t'r]. intuition. intuition. intuition. intuition. 
+    destruct s' as [s'l | s'r]. intuition.
+    eauto.
+  Qed.
+
+End RelLemmas.    
+
