coq/iso.v
@@ -1,0 +1,417 @@
+(****************************************************************************)
+(* Semantic isomorphisms of algebraically-indexed types                     *)
+(****************************************************************************)
+
+Require Import ssreflect ssrbool ssrfun seq.
+Require Import Relations Program.Equality.
+Require Import Rel syn Casts sem.
+Require Import FunctionalExtensionality.
+
+Set Implicit Arguments.
+Unset Strict Implicit.
+Import Prenex Implicits.
+
+(*==============================================================================================
+   TYPE ISOMORPHISMS
+
+   We define an isomorphism between types X and Y, written X ~= Y,
+   as a pair of maps i and j such that
+     forall psi, psi |= i : X -> Y
+     forall psi, psi |= j : Y -> X
+   and
+     forall psi, psi |= j o i = id : X -> X
+     forall psi, psi |= i o j = id : Y -> Y
+
+   We then show ~= is
+     (a) an equivalence relation
+     (b) a congruence, wrt all type constructors
+   and then prove
+     (a) units-independent isomorphisms, such as commutative of product, currying, etc
+     (b) units-dependent isomorphisms, as used in the proof of the Pi theorem in POPL'97.
+  ==============================================================================================*)
+
+Section Iso.
+
+Variable sig: SIG.
+Variable interpPrim: PrimType sig -> Type.
+
+Notation "| t |" := (interpTy interpPrim t).
+
+Definition Id D (t:Ty D) := fun (x:|t|) => x.
+Implicit Arguments Id [D]. 
+
+Variable ES: RelEnvSet interpPrim. 
+Variable A: seq (Ax sig). 
+Variable CLOSED: ClosedRelEnvSet A ES. 
+
+Notation "rho |= x == y :> t" := (@semTy sig interpPrim ES _ rho t x y) (at level 67, x at level 67, y at level 67).
+
+
+Open Scope Ty_scope.
+Definition iso D (X Y:Ty D) := exists i, exists j, 
+   (forall psi, psi |= i==i :> X --> Y) /\ 
+   (forall psi, psi |= j==j :> Y --> X) /\
+   (forall psi, psi |= (fun x => j(i(x))) == Id X :> X-->X) /\
+   (forall psi, psi |= (fun y => i(j(y))) == Id Y :> Y-->Y).
+
+Notation "X ~= Y" := (iso X Y) (at level 70).
+
+Section StandardIsos.
+
+Open Scope Ty_scope.
+
+Variable D : Ctxt sig.
+Variables W X Y Z : Ty D.
+Variable s : Srt sig. 
+Variables W' X' Y' Z' : Ty (s::D). 
+
+Axiom ENVDIF: forall D (psi: RelEnv interpPrim D) (p: PrimType sig) (exps: Sub (tyArity p) D), 
+  difunctional (psi p exps). 
+
+(*---------------------------------------------------------------------------
+   Type isomorphism is an equivalence relation
+   ---------------------------------------------------------------------------*)
+Lemma iso_refl : X ~= X.
+Proof. exists (fun x => x), (fun x => x) => /=//. Qed.
+
+Lemma iso_sym : X ~= Y -> Y ~= X.
+Proof. intros [i [j H] ]. exists j, i. intuition. Qed.
+
+Lemma iso_tran : X ~= Y -> Y ~= Z -> X ~= Z.
+Proof. move => H1 H2. destruct H1 as [i1 [j1 [H1a [H1b [H1c H1d] ] ] ] ]. simpl in *. 
+destruct H2 as [i2 [j2 [H2a [H2b [H2c H2d] ] ] ] ]. simpl in *. 
+exists (fun x => i2 (i1 (x))), (fun x => j1 (j2 (x))). 
+
+simpl. 
+split. intuition.  
+split. intuition.
+split. 
+
+intros psi x x' xx'.
+(* By logical interpretation of functions, we know i1 x ~ i1 x' *)  
+have H3 : semTy ES psi (i1 x) (i1 x'); auto.
+
+(* We now use difunctionality of the semantics *)
+assert (H4 := H2c psi (i1 x) (i1 x') H3). 
+assert (H5 := H1b psi (j2 (i2 (i1 x))) (i1 x') H4).
+assert (H6 := H1c psi x x' xx').
+assert (H7 := H1b psi (i1 x) (i1 x') H3).
+assert (DIF:= @sem_difunctional sig interpPrim ES A CLOSED ENVDIF D X psi).
+apply (DIF (j1(i1 x)) (j1(j2(i2(i1(x))))) x' (j1(i1 x')) H6 H5 H7).
+
+(* By logical interpretation of functions, we know j1 z ~ y1 z' *)
+intros psi z z' zz'.
+assert (H3 : semTy ES psi (j2 z) (j2 z')); auto.
+
+(* We now use difunctionality of the semantics *)
+assert (H4 := H1d psi (j2 z) (j2 z') H3).
+assert (H5 := H2a psi (i1 (j1 (j2 z))) (j2 z') H4).
+assert (H6 := H2d psi z z' zz').
+assert (H7 := H2a psi (j2 z) (j2 z') H3).
+assert (DIF := @sem_difunctional sig interpPrim ES A CLOSED ENVDIF D Z psi).
+unfold difunctional in DIF.
+apply (DIF (i2(j2 z)) (i2(i1(j1(j2 z)))) z' (i2(j2 z')) H6 H5 H7).
+Qed.
+
+(*---------------------------------------------------------------------------
+   Type isomorphism is a congruence
+   ---------------------------------------------------------------------------*)
+(* Product *)
+Lemma iso_prod_cong : W ~= X -> Y ~= Z -> W * Y ~= X * Z.
+Proof.
+  unfold iso, Id. simpl. 
+  intros WX YZ.
+  destruct WX as [Xi [Xj [Xihas_ty [Xjhas_ty [Xji Xij] ] ] ] ].
+  destruct YZ as [Yi [Yj [Yihas_ty [Yjhas_ty [Yji Yij] ] ] ] ].
+  
+  exists (fun p => (Xi p.1, Yi p.2)).
+  exists (fun p => (Xj p.1, Yj p.2)).
+  repeat (split; simpl; intuition).
+Qed.
+
+(* Arrow *)
+Lemma iso_arrow_cong (X1 X2 Y1 Y2 : Ty D) : X1 ~= X2 -> Y1 ~= Y2 -> X1 --> Y1 ~= X2 --> Y2.
+Proof.
+  unfold iso, Id. simpl. 
+  intros X1X2 Y1Y2.
+  destruct X1X2 as [Xi [Xj [Xihas_ty [Xjhas_ty [Xji Xij ] ] ] ] ].
+  destruct Y1Y2 as [Yi [Yj [Yihas_ty [Yjhas_ty [Yji Yij ] ] ] ] ].
+
+  exists (fun f => fun x => Yi (f (Xj x))).
+  exists (fun f => fun x => Yj (f (Xi x))).
+  repeat (split; simpl; intuition).
+Qed.
+
+(* Sum *)
+Lemma iso_sum_cong (X1 X2 Y1 Y2 : Ty D) : X1 ~= X2 -> Y1 ~= Y2 -> X1 + Y1 ~= X2 + Y2.
+Proof.
+  unfold iso, Id. simpl. 
+  intros X1X2 Y1Y2.
+  destruct X1X2 as [Xi [Xj [Xihas_ty [Xjhas_ty [Xji Xij ] ] ] ] ].
+  destruct Y1Y2 as [Yi [Yj [Yihas_ty [Yjhas_ty [Yji Yij ] ] ] ] ].
+
+  exists (fun s => match s with inl l => inl _ (Xi l) | inr r => inr _ (Yi r) end).
+  exists (fun s => match s with inl l => inl _ (Xj l) | inr r => inr _ (Yj r) end).
+  split.
+  intro psi.
+  case => x. case => y; intuition. case => x'; intuition. 
+  split.
+  intro psi.
+  case => x. case => y; intuition. case => x'; intuition. 
+  split.  
+  intro psi.
+  case => x. case => y; intuition. case => y; intuition.
+  intro psi. 
+  case => x. case => y; intuition. case => y; intuition.
+Qed.
+
+Lemma iso_all_cong : X' ~= Y' -> TyAll X' ~= TyAll Y'.
+Proof.
+  unfold iso, Id. simpl. 
+  intros X'Y'.
+  destruct X'Y' as [i [j [ihas_ty [jhas_ty [ji ij ] ] ] ] ].
+
+  exists i, j; intuition.   
+Qed.
+
+(*---------------------------------------------------------------------------
+   Pushing quantifiers through type constructors
+   ---------------------------------------------------------------------------*)
+(* Arrows *)
+Lemma iso_all_arrow : TyAll (apSubTy (pi _ _) X --> Y') ~= (X --> TyAll Y').
+Proof.
+  unfold iso, Id. simpl. 
+  exists (fun f x => f (up _ x)).
+  exists (fun f x => f (dn x)).  
+  split.
+  intros psi f f' ff' x x' xx' psi' H EXT.
+  apply (ff' _ H EXT).  
+  have SS:= @semSubst sig interpPrim ES A CLOSED D X (s::D) (pi D s) psi' H x x'.  
+  rewrite SS. 
+  rewrite /ext in EXT. 
+  rewrite EXT. 
+  apply xx'. 
+
+  split.
+  intros psi f f' ff' psi' H EXT x x' xx'. 
+  have SS:= @semSubst sig interpPrim ES A CLOSED D X (s::D) (pi D s) psi' H (dn x) (dn x').  
+  specialize (ff' (dn x) (dn x')). 
+  apply ff' => //. rewrite EXT in SS. rewrite -SS. 
+  rewrite 2!updn. apply xx'. 
+
+  split.
+  intros psi f f' ff' psi' H EXT x x' xx'.
+  rewrite updn.
+  intuition.
+
+  intros psi f f' ff' x x' x'' psi' H EXT.
+  rewrite dnup. intuition.
+Qed.
+
+(* Products *)
+Lemma iso_all_prod : TyAll (X' * Y') ~= TyAll X' * TyAll Y'. 
+Proof.
+  unfold iso, Id. simpl.
+  exists (fun p => p). 
+  exists (fun p => p). 
+  split. 
+  intros. split. intros psi' ESS EXT. specialize (H psi' ESS EXT). apply (proj1 H). 
+  intros psi' ESS EXT. apply (proj2 (H psi' ESS EXT)). 
+  split.
+  intros. destruct H.  auto. 
+  split. auto. auto. 
+Qed.
+
+(* Elimination of redundant quantifiers *)
+Lemma iso_all_redundant : TyAll (apSubTy (pi _ s) X) ~= X.
+Proof.
+  unfold iso, Id. simpl. 
+  exists (fun x => dn x). 
+  exists (fun x => up _ x).  
+  split.
+  intros psi x x' xx'.
+Admitted.
+(* We need a way of lifting RelEnv D to RelEnv (s::D) *)
+(*  specialize (xx' (psi o DOWN _) (SEnvDown _)). 
+  assert (DOWN _ o @SHIFT n = Hom.Id). apply HomExtensional. intros u. simpl. rewrite downShift. auto.  
+  rewrite <- (Compose_id_r psi). rewrite <- H. rewrite Compose_assoc. 
+  admit. (*rewrite SEnvSubstSem. repeat rewrite updn. auto.  *)
+  
+  split. 
+  intros psi x x' xx' psi' ext.  rewrite <- SEnvSubstSem. rewrite (proj1 (SEnvExtendsDef _ _) ext). auto. 
+  
+  split. 
+  intros psi x x' xx' psi' ext.  rewrite updn. apply xx'. auto. 
+  intros psi x x' xx'. rewrite dnup. auto. 
+Qed.*)
+
+
+(*---------------------------------------------------------------------------
+   Arithmetic-style isomorphisms
+   ---------------------------------------------------------------------------*)
+(* Product is commutative *)
+Lemma iso_prod_comm : X*Y ~= Y*X.
+  exists (fun p => (p.2,p.1)).
+  exists (fun p => (p.2,p.1)).
+  simpl; intuition. 
+Qed.
+
+(* Product is associative *)
+Lemma iso_prod_assoc : X*(Y*Z) ~= (X*Y)*Z.
+  exists (fun p => ((p.1, p.2.1), p.2.2)).
+  exists (fun p => (p.1.1, (p.1.2, p.2))).
+  simpl; intuition.
+Qed.
+
+(* Unit is a right unit for product *)
+Lemma iso_prod_unit : X*(TyUnit _) ~= X.
+  exists (fun p => p.1).
+  exists (fun x => (x,tt)).
+  simpl;intuition.
+Qed.
+
+(* Sum is commutative *)
+Lemma iso_sum_comm : X+Y ~= Y+X.
+  exists (fun s  => match s with inl x => @inr _ _ x | inr y => @inl _ _ y end).
+  exists (fun s => match s with inl x => @inr _ _ x | inr y => @inl _ _ y end).
+  simpl. simpl in *. 
+  split. intro psi. destruct x'. destruct y'; intuition. destruct y'; intuition.
+  split. intro psi. destruct x'. destruct y'; intuition. destruct y'; intuition.
+  split. intro psi. destruct x'. destruct y'; intuition. destruct y'; intuition.
+         destruct x'. destruct y'; intuition. by destruct y'. 
+Qed.
+
+(* Sum is associative *)
+Lemma iso_sum_assoc : X+(Y+Z) ~= (X+Y)+Z.
+Proof.
+  exists (fun s => 
+          match s with 
+          | inl x => @inl _ _ (@inl _ _ x) 
+          | inr yz => match yz with inl y => @inl _ _ (@inr _ _ y) | inr z => @inr _ _ z end end).
+  exists (fun s  =>
+          match s with
+          | inl xy => match xy with inl x => @inl _ _ x | inr y => @inr _ _ (@inl _ _ y) end
+          | inr z => @inr _ _ (@inr _ _ z) end).
+  simpl. 
+  split. intro psi. destruct x'. destruct y'; intuition. destruct y'; intuition.
+    destruct s1. destruct s0; intuition. destruct s0; intuition. 
+  split. intro psi. destruct x'. destruct y'; intuition. destruct s1; intuition. destruct s0; intuition. destruct s0; intuition.
+  destruct y'; intuition.
+
+  split. intro psi. destruct x'.  destruct y'; intuition. destruct y'; intuition. destruct s0; intuition. 
+  destruct x'; intuition.
+Qed.
+
+
+Definition Weird : interpTy interpPrim X + False -> interpTy interpPrim X. 
+intros. destruct X0. assumption. done. 
+Defined.
+
+(* Void is a right unit for sum *)
+(*
+Lemma iso_sum_zero : X + Void ~= X.
+Proof. 
+  unfold iso. fold usem.
+  exists Weird. 
+  exists (fun x : usem X => @inl _ _ x).
+  split. Unfoldsem2.  intros psi x y. destruct x; destruct y. simpl. auto. destruct f. destruct f. destruct f. 
+  split. Unfoldsem2. intros. auto. 
+  split. Unfoldsem2. intros. destruct x; destruct y; auto. destruct f.
+  Unfoldsem2.  intros. simpl. auto. 
+Qed.
+*)
+
+(* Product distributes over sum *)
+(* Annoyingly, can't get proof through if we pattern match on product; need to use fst/snd *)
+Lemma iso_prod_sum : X*(Y+Z) ~= X*Y + X*Z.
+  exists (fun p  =>
+        match snd p with
+        | inl y => inl _ (p.1, y)
+        | inr z => inr _ (p.1, z) end).
+  exists (fun s =>
+        match s with
+        | inl p => (p.1, inl _ p.2)
+        | inr p => (p.1, inr _ p.2) end).
+
+  simpl. 
+  split.
+  
+  intros psi [p1 p2] [q1 q2] H.
+  simpl.   
+  destruct p2; destruct q2; intuition. 
+  
+  split. 
+  
+  intros psi s1 s2 H. 
+  destruct s1; destruct s2; intuition. 
+
+  split. 
+
+  destruct x'; intuition. 
+  destruct x'; intuition. 
+Qed.
+
+(* Exponential of a sum *)
+Lemma iso_sum_arrow : (X+Y)-->Z ~= (X-->Z)*(Y-->Z).
+Proof.
+  exists (fun f =>
+         (fun a => f (@inl _ _ a), fun b => f (@inr _ _ b))).
+  exists (fun p =>
+          fun s => 
+          match s with inl a => (fst p) a | inr b => (snd p) b end).
+
+  simpl. 
+
+  split.
+  intros psi f g. simpl. intuition. 
+  split. intros psi f g fg. simpl. case. move => a.  case; intuition. move => b. case; intuition. 
+  split. intuition. 
+  split. intuition. 
+  intuition. 
+Qed.
+
+(* Currying *)
+Lemma iso_curry : (X*Y) --> Z ~= X --> Y --> Z.
+Proof.
+  exists (fun g => fun x => fun y => g (x,y)). simpl. 
+  exists (fun f => fun p  => f (fst p) (snd p)).
+  simpl; intuition. 
+Qed.
+
+Lemma iso_swaparg : X --> Y --> Z ~= Y --> X --> Z.
+Proof.
+  exists (fun f => fun x => fun y => f y x).
+  exists (fun f => fun x => fun y => f y x).
+  simpl; intuition. 
+Qed.
+
+(* Exponential of unit *)
+Lemma iso_arrow_unit : X --> TyUnit _ ~= TyUnit _.
+Proof.
+  exists (fun f => tt).
+  exists (fun _ : unit => fun _ => tt).
+  simpl; intuition. 
+Qed.
+
+(* Unit exponential *)
+Lemma iso_unit_arrow : TyUnit _ --> X ~= X.
+Proof.
+  exists (fun f  => f tt).
+  exists (fun x  => fun _:unit => x). 
+  simpl; intuition. 
+Qed.
+
+(* Exponential of product *)
+Lemma iso_arrow_prod : Z --> (X*Y) ~= (Z-->X) * (Z-->Y).
+Proof.
+  exists (fun f  => (fun z => fst (f z), fun z => snd (f z))).
+  exists (fun p  => fun z => (fst p z, snd p z)).
+  simpl; intuition. 
+  simpl; intuition; apply (H _ _ H0).  
+  simpl; intuition; apply (H _ _ H0).  
+Qed.
+
+End StandardIsos.
+
+
+End Iso.
